bedrock2/src/bedrock2/BasicC64Semantics.v
@@ -5,19 +5,20 @@ Require Import coqutil.Word.Interface coqutil.Map.SortedListWord.
 Require coqutil.Word.Naive.
 Require Export coqutil.Word.Bitwidth64.
 
-#[global] Instance word: word.word 64 := Naive.word64.
-#[global] Instance mem: Interface.map.map word Byte.byte := SortedListWord.map _ _.
-#[global] Instance locals: Interface.map.map String.string word := SortedListString.map _.
-#[global] Instance env: Interface.map.map String.string (list String.string * list String.string * cmd) :=
+#[export] Existing Instances Bitwidth64.BW64.
+#[export] Instance word: word.word 64 := Naive.word64.
+#[export] Instance mem: Interface.map.map word Byte.byte := SortedListWord.map _ _.
+#[export] Instance locals: Interface.map.map String.string word := SortedListString.map _.
+#[export] Instance env: Interface.map.map String.string (list String.string * list String.string * cmd) :=
   SortedListString.map _.
-#[global] Instance ext_spec: ExtSpec := fun _ _ _ _ _ => False.
+#[export] Instance ext_spec: ExtSpec := fun _ _ _ _ _ => False.
 
 Arguments word: simpl never.
 Arguments mem: simpl never.
 Arguments locals: simpl never.
 Arguments env: simpl never.
 
-#[global] Instance weaken_ext_spec trace m0 act args :
+#[export] Instance weaken_ext_spec trace m0 act args :
   Morphisms.Proper
     (Morphisms.respectful
        (Morphisms.pointwise_relation Interface.map.rep
@@ -30,16 +31,16 @@ Proof.
   assumption.
 Qed.
 
-#[global] Instance localsok: coqutil.Map.Interface.map.ok locals := SortedListString.ok _.
-#[global] Instance envok: coqutil.Map.Interface.map.ok env := SortedListString.ok _.
-#[global] Instance mapok: coqutil.Map.Interface.map.ok mem := SortedListWord.ok Naive.word64 _.
-#[global] Instance wordok: coqutil.Word.Interface.word.ok word := Naive.word64_ok.
+#[export] Instance localsok: coqutil.Map.Interface.map.ok locals := SortedListString.ok _.
+#[export] Instance envok: coqutil.Map.Interface.map.ok env := SortedListString.ok _.
+#[export] Instance mapok: coqutil.Map.Interface.map.ok mem := SortedListWord.ok Naive.word64 _.
+#[export] Instance wordok: coqutil.Word.Interface.word.ok word := Naive.word64_ok.
 Add Ring wring : (Properties.word.ring_theory (word := word))
       (preprocess [autorewrite with rew_word_morphism],
        morphism (Properties.word.ring_morph (word := word)),
        constants [Properties.word_cst]).
 
-#[global] Instance ext_spec_ok : ext_spec.ok ext_spec.
+#[export] Instance ext_spec_ok : ext_spec.ok ext_spec.
 Proof.
   constructor; intros; try contradiction.
   apply weaken_ext_spec.
